zoo/common/format: Change hole separator to ";" and introduce variable forwarding.

theories/zoo/common/format.v
@@ -17,19 +17,25 @@ Definition format_env :=
   gmap string string.
 Implicit Types env : format_env.
 
-#[local] Definition parse_binding str :=
-  let '(var, val) := split_on "=" str in
-  let val := default var val in
-  (var, val).
-
-Definition format_env_of_bindings bdgs : format_env :=
-  list_to_map bdgs.
-Definition format_env_of_strings strs :=
-  format_env_of_bindings (parse_binding <$> strs).
-Definition format_env_of_string str :=
-  format_env_of_strings (String.words str).
-
 Module parse.
+  Notation assign :=
+    "="%char.
+  Notation sep :=
+    ";"%char.
+  Notation hole_beg :=
+    "{"%char.
+  Notation hole_end :=
+    "}"%char.
+  Notation forward_beg :=
+    "/"%char.
+  Notation forward_end :=
+    "/"%char.
+
+  Definition binding str :=
+    let '(var, val) := split_on assign str in
+    let val := default var val in
+    (var, val).
+
   Inductive insideness :=
     | Inside
     | Outside.
@@ -38,7 +44,7 @@ Module parse.
     match str with
     | "" =>
         Some (String.rev res)
-    | String "{" str =>
+    | String hole_beg str =>
         hole env str res ""
     | String chr str =>
         go env str (String chr res)
@@ -47,16 +53,18 @@ Module parse.
     match str with
     | "" =>
         None
-    | String "{" str =>
+    | String hole_beg str =>
         hole_variable env str res acc ""
-    | String "}" str =>
+    | String forward_beg str =>
+        hole_forward env str res acc ""
+    | String hole_end str =>
         match env !! String.rev acc with
         | None =>
             go env str (acc +:+ res)
         | Some val =>
             go env str (String.rev val +:+ res)
         end
-    | String "=" str =>
+    | String sep str =>
         match env !! String.rev acc with
         | None =>
             hole' env str res ""
@@ -70,11 +78,13 @@ Module parse.
     match str with
     | "" =>
         None
-    | String "{" str =>
+    | String hole_beg str =>
         hole_variable env str res acc ""
-    | String "}" str =>
+    | String forward_beg str =>
+        hole_forward env str res acc ""
+    | String hole_end str =>
         go env str (acc +:+ res)
-    | String "=" str =>
+    | String sep str =>
         hole_finish env str (acc +:+ res) Outside
     | String chr str =>
         hole' env str res (String chr acc)
@@ -83,7 +93,7 @@ Module parse.
     match str with
     | "" =>
         None
-    | String "}" str =>
+    | String hole_end str =>
         match env !! String.rev var with
         | None =>
             hole_next env str res Outside
@@ -93,13 +103,27 @@ Module parse.
     | String chr str =>
         hole_variable env str res acc (String chr var)
     end
+  with hole_forward env str res acc var :=
+    match str with
+    | "" =>
+        None
+    | String forward_end str =>
+        match env !! String.rev var with
+        | None =>
+            hole' env str res acc
+        | Some val =>
+            hole' env str res (String.rev val +:+ String assign var +:+ acc)
+        end
+    | String chr str =>
+        hole_forward env str res acc (String chr var)
+    end
   with hole_finish env str res state :=
     match str with
     | "" =>
         None
-    | String "{" str =>
+    | String hole_beg str =>
         hole_finish env str res Inside
-    | String "}" str =>
+    | String hole_end str =>
         if state is Inside then
           hole_finish env str res Outside
         else
@@ -111,25 +135,31 @@ Module parse.
     match str with
     | "" =>
         None
-    | String "{" str =>
+    | String hole_beg str =>
         hole_next env str res Inside
-    | String "}" str =>
+    | String hole_end str =>
         if state is Inside then
           hole_next env str res Outside
         else
           go env str res
-    | String "=" str =>
+    | String sep str =>
         hole' env str res ""
     | String _ str =>
         hole_next env str res state
     end.
-
-  Definition main env str :=
+  Definition format env str :=
     go env str "".
 End parse.
 
+Definition format_env_of_bindings bdgs : format_env :=
+  list_to_map bdgs.
+Definition format_env_of_strings strs :=
+  format_env_of_bindings (parse.binding <$> strs).
+Definition format_env_of_string str :=
+  format_env_of_strings (String.words str).
+
 Definition format fmt env :=
-  parse.main env fmt.
+  parse.format env fmt.
 
 Goal format "{}" ∅ = Some "".
 Proof. reflexivity. Qed.
@@ -144,33 +174,33 @@ Proof. reflexivity. Qed.
 Goal format "{1} {2}" {["1":="one";"2":="two"]} = Some "one two".
 Proof. reflexivity. Qed.
 
-Goal format "{1=∅}" ∅ = Some "∅".
+Goal format "{1;∅}" ∅ = Some "∅".
 Proof. reflexivity. Qed.
-Goal format "{1=∅}" {["1":="one"]} = Some "one".
-Proof. reflexivity. Qed.
-
-Goal format "{1=}" ∅ = Some "".
-Proof. reflexivity. Qed.
-Goal format "{1=}" {["1":="one"]} = Some "one".
+Goal format "{1;∅}" {["1":="one"]} = Some "one".
 Proof. reflexivity. Qed.
 
-Goal format "{({1})=∅}" ∅ = Some "∅".
+Goal format "{1;}" ∅ = Some "".
 Proof. reflexivity. Qed.
-Goal format "{({1})=∅}" {["1":="one"]} = Some "(one)".
-Proof. reflexivity. Qed.
-
-Goal format "{({1})=({2})}" ∅ = Some "".
-Proof. reflexivity. Qed.
-Goal format "{({1})=({2})}" {["1":="one"]} = Some "(one)".
-Proof. reflexivity. Qed.
-Goal format "{({1})=({2})}" {["2":="two"]} = Some "(two)".
+Goal format "{1;}" {["1":="one"]} = Some "one".
 Proof. reflexivity. Qed.
 
-Goal format "{({1})=({2})=∅}" ∅ = Some "∅".
+Goal format "{({1});∅}" ∅ = Some "∅".
 Proof. reflexivity. Qed.
-Goal format "{({1})=({2})=∅}" {["1":="one"]} = Some "(one)".
+Goal format "{({1});∅}" {["1":="one"]} = Some "(one)".
 Proof. reflexivity. Qed.
-Goal format "{({1})=({2})=∅}" {["2":="two"]} = Some "(two)".
+
+Goal format "{({1});({2})}" ∅ = Some "".
+Proof. reflexivity. Qed.
+Goal format "{({1});({2})}" {["1":="one"]} = Some "(one)".
+Proof. reflexivity. Qed.
+Goal format "{({1});({2})}" {["2":="two"]} = Some "(two)".
+Proof. reflexivity. Qed.
+
+Goal format "{({1});({2});∅}" ∅ = Some "∅".
+Proof. reflexivity. Qed.
+Goal format "{({1});({2});∅}" {["1":="one"]} = Some "(one)".
+Proof. reflexivity. Qed.
+Goal format "{({1});({2});∅}" {["2":="two"]} = Some "(two)".
 Proof. reflexivity. Qed.
 
 Goal format "{{1}-{2}}" ∅ = Some "".
@@ -182,11 +212,16 @@ Proof. reflexivity. Qed.
 Goal format "{{1}-{2}}" {["1":="one";"2":="two"]} = Some "one-two".
 Proof. reflexivity. Qed.
 
-Goal format "{{1}-{2}=∅}" ∅ = Some "∅".
+Goal format "{{1}-{2};∅}" ∅ = Some "∅".
 Proof. reflexivity. Qed.
-Goal format "{{1}-{2}=∅}" {["1":="one"]} = Some "∅".
+Goal format "{{1}-{2};∅}" {["1":="one"]} = Some "∅".
 Proof. reflexivity. Qed.
-Goal format "{{1}-{2}=∅}" {["2":="two"]} = Some "∅".
+Goal format "{{1}-{2};∅}" {["2":="two"]} = Some "∅".
 Proof. reflexivity. Qed.
-Goal format "{{1}-{2}=∅}" {["1":="one";"2":="two"]} = Some "one-two".
+Goal format "{{1}-{2};∅}" {["1":="one";"2":="two"]} = Some "one-two".
+Proof. reflexivity. Qed.
+
+Goal format "{/1/}" {["1":="one"]} = Some "1=one".
+Proof. reflexivity. Qed.
+Goal format "{/1/}" ∅ = Some "".
 Proof. reflexivity. Qed.
