theories/zoo_saturn/mpmc_bqueue.v
@@ -140,7 +140,7 @@ Section mpmc_bqueue_G.
       #H{}_header &
       #H{}_index &
       #Hhistory_at_{} &
-      {{front}#Hfront_lb_{}=_}
+      {{front}#Hfront_lb_{};_}
     )".
 
   #[local] Definition waiter_au γ (Ψ : bool → iProp Σ) : iProp Σ :=
